short example actually short

theories/examples/example.v
@@ -38,258 +38,63 @@ Module Type SignatureDefs.
     Definition Seed : choice_type := chFin(mkpos pos_n).
     Definition SecKey : choice_type := chFin(mkpos pos_n).
     Definition PubKey : choice_type := chFin(mkpos pos_n).
+    
+    #[local] Open Scope package_scope.
+
+    Parameter KeyGen : ∀ (sd : Seed), (SecKey × PubKey).
 
 End SignatureDefs.
 
-Module Type SignatureAlgorithms (π : SignatureDefs).
-  
-  Import π.  
-  #[local] Open Scope package_scope.
-
-  Parameter KeyGen : ∀ (sd : Seed), (SecKey × PubKey).
-    
-End SignatureAlgorithms.
-
-Module RemoteAttestation (π : SignatureDefs)
-  (Alg : SignatureAlgorithms π).
+Module RemoteAttestation (π : SignatureDefs).
 
   Import π.
-  Import Alg.
-  #[local] Open Scope package_scope.
 
-  Notation " 'pubkey "    := PubKey      (in custom pack_type at level 2).
-  Notation " 'pubkey "    := PubKey      (at level 2): package_scope.
-  Notation " 'seckey "    := SecKey      (in custom pack_type at level 2).
-  Notation " 'seckey "    := SecKey      (at level 2): package_scope.  
-  Notation " 'seed "      := Seed        (in custom pack_type at level 2).
-  Notation " 'seed "      := Seed        (at level 2): package_scope.
-
-  Definition chSet t := chMap t 'unit.
-  Notation " 'set t " := (chSet t) (in custom pack_type at level 2).
-  Notation " 'set t " := (chSet t) (at level 2): package_scope.
-
-  Definition tt := Datatypes.tt.
-
+  Notation " 'pubkey "    := PubKey      (in custom pack_type at level 2) : package_scope. 
+  Notation " 'seckey "    := SecKey      (in custom pack_type at level 2) : package_scope.  
+  Notation " 'seed "      := Seed        (in custom pack_type at level 2) : package_scope.
+  
   Definition pk_loc      : Location := (PubKey    ; 0%N).
   Definition sk_loc      : Location := (SecKey    ; 1%N).
-
-  Definition key_gen   : nat := 42. (* routine to get the public key *)
-
+  Definition key_gen   : nat := 42. 
   Definition KeyGen_locs := fset [:: pk_loc ; sk_loc ]. 
+  Definition KG_interface := [interface #val #[key_gen] : 'seed → 'pubkey ].
 
-  Definition Ideal_interface := [interface
-  #val #[key_gen] : 'unit → 'pubkey 
-  ].
-
-  Definition Key_Gen_real :
+  Definition KG_real :
   package KeyGen_locs
     [interface]
-    [interface #val #[key_gen] : 'unit → 'pubkey ].
+    KG_interface
   :=
   [package
-    #def  #[key_gen] (_ : 'unit) : 'pubkey
+    #def  #[key_gen] (sd : 'seed) : 'pubkey
     {
-    let (sk,pk) := KeyGen2 sd in
-    #put pk_loc := pk ;;
-    #put sk_loc := sk ;;
+    let (sk,pk) := KeyGen sd in
     ret pk
     }
   ].
 
-  Definition Sig_ideal :
-  package Signature_locs
+  Definition KG_ideal :
+  package KeyGen_locs
     [interface]
-    Sign_interface
+    KG_interface
   :=
   [package
-    #def  #[get_pk] (_ : 'unit) : 'pubkey
+    #def  #[key_gen] (sd : 'seed) : 'pubkey
     {
-      pk ← get pk_loc ;;
-      ret pk
-    } ;
-    #def #[sign] ( '(msg,sd) : 'message × 'seed) : 'signature
-    {
-      (*'(sk, pk) ← KeyGen2 sd ;;*)
-      let (sk,pk) := KeyGen2 sd in
-      #put pk_loc := pk ;;
-      #put sk_loc := sk ;;      
-      sig ← Sign sk msg ;; 
-      S ← get sign_loc ;; 
-      #put sign_loc := setm S (sig, msg) tt ;;
-      ret sig
-    };
-    #def #[verify_sig] ( '(sig,msg) : 'signature × 'message) : 'bool
-    {
-      S ← get sign_loc ;;
-      ret ( (sig,msg) \in domm S)      
+    let (sk,pk) := KeyGen sd in
+    ret pk
     }
   ].
-
-  Definition ɛ_sig A := AdvantageE Sig_real Sig_ideal A. 
 
   Definition mkpair {Lt Lf E}
   (t: package Lt [interface] E) (f: package Lf [interface] E):
   loc_GamePair E := fun b => if b then {locpackage t} else {locpackage f}.  
 
-  Definition Sig_unforg := @mkpair Signature_locs Signature_locs Sign_interface Sig_real Sig_ideal.
+  Definition KG_ind := @mkpair KeyGen_locs KeyGen_locs KG_interface KG_real KG_ideal.
 
-  Definition i_challenge := #|Challenge|.
-  Definition i_challenge_pos : Positive i_challenge.
-  Proof.
-    unfold i_challenge.
-    apply Challenge_pos.
-  Qed.
-
-  Definition Aux :
-  package (fset [:: sign_loc ; pk_loc ; attest_loc ])
-  [interface
-  #val #[get_pk] : 'unit → 'pubkey ;
-  #val #[sign] : ('message × 'seed)  → 'signature ;
-  #val #[verify_sig] : ('signature × 'message) → 'bool
-  ]
-  [interface
-  #val #[get_pk] : 'unit → 'pubkey ;
-  #val #[attest] : ('challenge × ('state × 'seed)) → 'signature ;
-  #val #[verify_att] : ( ('challenge × 'state) × 'signature) → 'bool
-  ]
-  :=
-  [package
-    #def #[get_pk] (_ : 'unit) : 'pubkey
-    {
-      pk ← get pk_loc ;;
-      ret pk
-    } ;
-    #def #[attest] ( '(chal,(state,sd)) : ('challenge × ('state × 'seed))) : 'signature
-    {
-      #import {sig #[sign] : ('message  × 'seed) → 'signature } as sign ;;
-      let msg := Hash state chal in
-      att ← sign (msg,sd) ;;
-      (*#put attest_loc := att ;;*)
-      ret att
-    } ;
-    #def #[verify_att] ('(chal, state, att) : ('challenge × 'state) × 'signature) : 'bool
-    {
-      #import {sig #[verify_sig] : ('signature × 'message) → 'bool } as verify ;;
-      let msg := Hash state chal in
-      pk ← get pk_loc ;;
-      verify (att,msg) 
-    }
-  ].
-
-(* Encryption algorithm *)
- 
-  Definition Att_real :
-  package Attestation_locs
-    [interface]
-    Att_interface
-  :=
-  [package
-    #def  #[get_pk] (_ : 'unit) : 'pubkey
-    {
-      pk ← get pk_loc  ;;
-      ret pk
-    } ;
-    #def #[attest] ( '(chal,(state,sd)) : 'challenge × ('state × 'seed)) : 'signature
-    {
-      (*'(sk, pk) ← KeyGen2 sd ;;*)
-      let (sk,pk) := KeyGen2 sd in
-      #put pk_loc := pk ;;
-      #put sk_loc := sk ;;
-      att ← Attest sk chal state ;;
-      ret att
-    };
-    #def #[verify_att] ('(chal, state, att) : ('challenge × 'state) × 'signature) : 'bool
-    {
-      pk ← get pk_loc  ;;
-      bool ← Ver_att pk att chal state ;;
-      ret bool
-    }
-  ].
-
-  Definition Att_ideal :
-  package Attestation_locs
-    [interface]
-    Att_interface
-  :=
-  [package
-    #def  #[get_pk] (_ : 'unit) : 'pubkey
-    {
-      pk ← get pk_loc ;;
-      ret pk
-    } ;
-    #def #[attest] ( '(chal,(state,sd)) : 'challenge × ('state × 'seed)) : 'attest
-    {
-      A ← get attest_loc ;;
-      (*'(sk, pk) ← KeyGen2 sd ;;*)
-      let (sk,pk) := KeyGen2 sd in
-      #put pk_loc := pk ;;
-      #put sk_loc := sk ;;
-      att ← Attest sk chal state ;;      
-      #put attest_loc := setm A ( chal, state, att ) tt ;; 
-      ret att
-    };
-    #def #[verify_att] ('(chal, state, att) : ('challenge × 'state) × 'attest) : 'bool
-    {
-      A ← get attest_loc ;;
-      ret ( (chal, state, att) \in domm A )
-    }
-  ].
-
-  Definition ɛ_att A := AdvantageE Att_real Att_ideal A.
-
-  Definition Att_unforg := mkpair Att_real Att_ideal.
-
-  Lemma sig_real_vs_att_real_true :
-  Att_unforg true ≈₀ Aux ∘ Sig_unforg true.
+  Lemma KG_real_vs_KG_true :
+  KG_ind true ≈₀ KG_ind false.
   Proof.
     eapply eq_rel_perf_ind_eq.
     simplify_eq_rel x.
     all: ssprove_code_simpl. 
-    - eapply rpost_weaken_rule.
-      1: eapply rreflexivity_rule.
-      move => [a1 h1] [a2 h2] [Heqa Heqh]. 
-      intuition auto.
-    - (*rewrite !cast_fun_K.*)
-      destruct x.
-      destruct s0.
-      ssprove_sync_eq.
-      ssprove_sync_eq.
-      ssprove_code_simpl_more.
-      eapply rsame_head_alt. 
-      simpl.
-      eapply rreflexivity_rule.
-
-
-
-      eapply rreflexivity_rule.
-      ssprove_sync_eq.
-      ssprove_code_simpl_more.
-      eapply rsame_head_alt.          
-      ssprove_sync.  
-      ssprove_sync_eq. 
-      
-    ssprove_swap_lhs 0%N. 
-    Admitted.
-  (*Qed.*)
-
-  Lemma sig_ideal_vs_att_ideal_true :
-  Att_ideal ≈₀ Aux ∘ Sig_ideal.
-  Proof.
-    eapply eq_rel_perf_ind_eq.
-    simplify_eq_rel m.
-    all: ssprove_code_simpl.
-    Admitted.
-  (*Qed.*)
-
-  Theorem RA_unforg LA A :
-  ∀ LA A,
-    ValidPackage LA [interface
-    #val #[get_pk] : 'unit → 'pubkey ;
-    #val #[sign] : ('challenge × 'state) → 'attest ;
-    #val #[verify_sig] : ( ('challenge × 'state) × 'attest) → 'bool
-    ] A_export A →
-    fdisjoint LA (sig_real_vs_att_real_true).(locs) →
-    fdisjoint LA (sig_ideal_vs_att_ideal_true).(locs) →
-    Advantage Att_unforg <= Advantage Sig_unforg.
-Proof.
-  
+    eapply rsame_head_alt. 
